Replace aborted proofs with completed proofs using additional assumptions, for unsigned integer side-conditions For the ERC-20 wrapped ether smart contract

Chapter-6-Case-Study-ERC-20-Wrapped-Ether-Token/proofs/ObjERC20WrappedEthCodeProofs.v
@@ -12,12 +12,17 @@ Existing Instance GlobalLayerSpec.
 Existing Instances CONTRACT_overlay_spec.
 
 Context {memModelOps : MemoryModelOps mem}.
+Context (HCompatDataOps : CompatDataOps global_abstract_data_type).
 
 
 Ltac code_proofs_auto :=
     intros;
     unfold synth_func_obligation;
     repeat (split; auto).
+
+Definition toZ : unpair_ft (tint_Z_bounded Int256.modulus) -> Z := id.
+Definition etherToWei (ether : Z) : Z := ether * (10 ^ 18).
+Definition unattainableWeiAmount := etherToWei (10 ^ 20).
 
 Lemma ERC20WrappedEth_constructor_vc me d :
     high_level_invariant d ->
@@ -132,13 +137,23 @@ code_proofs_auto.
 Qed.
 
 Lemma ERC20WrappedEth_transfer_vc a0 a1 me d :
+    (forall a,
+      Int256Tree.get_default 0 a (ERC20WrappedEth_wrapped d)
+        < unattainableWeiAmount) ->
+    (toZ a1 < unattainableWeiAmount) ->
     ht_ft_cond a0 -> ht_valid_ft_cond a0 ->
     ht_ft_cond a1 -> ht_valid_ft_cond a1 ->
     high_level_invariant d ->
     synth_func_cond ERC20WrappedEth_transfer ERC20WrappedEth_transfer_wf
                     a0 a1 me d.
 Proof.
+intros Hextra1 Hextra2.
 intros.
+unfold _tp_type_pair in *.
+unfold unpair_ft in *.
+unfold _tp_type_pair in *.
+simpl in *.
+unfold Z32 in a1.
 remember a0 as _to. remember a1 as _value. 
 clear a0 a1 Heq_to Heq_value.
 unfold Z32 in _value. 
@@ -149,8 +164,28 @@ repeat split.
 - subst.
   simpl in *.
   inversion H9.
-  shelve.
-  - remember ((@SpecTree.get
+  inversion H8.
+  destruct(MachineModel.me_callvalue me =? 0) eqn:Case; [|simpl in H7; inversion H7].
+  simpl in H7. inversion H7.
+  destruct(Int256.eq (MachineModel.me_caller me) _to) eqn:SCase;
+    [simpl in H6; inversion H6|].
+  simpl in H6. inversion H6.
+  destruct(Int256.eq (MachineModel.me_caller me)
+  (MachineModel.me_address me)) eqn:SSCase; [simpl in H5; inversion H5|].
+  simpl in H5. inversion H5.
+  destruct(_value >=? 0) eqn:SSSCase; [|simpl in H4; inversion H4].
+  simpl in H4. inversion H4.
+  subst.
+  pose proof (Hextra1 _to). subst.
+  unfold Int256.modulus, two_power_nat. simpl.
+  unfold toZ, id in Hextra2.
+  clear -Hextra2 H11.
+  unfold Z_bounded in *.
+  remember (@Int256Tree.get_default Z Z0 _to (ERC20WrappedEth_wrapped m5)) as y.
+  unfold unattainableWeiAmount, etherToWei in *.
+  lia.
+  -
+  remember ((@SpecTree.get
   (param_env
      (@cons hyper_type_pair int_U_pair
         (@cons hyper_type_pair int_Z32_pair (@nil hyper_type_pair)))
@@ -173,7 +208,7 @@ repeat split.
   destruct (v >=? STORED_VALUE) eqn:Case; [|inversion H10]. simpl in *. (* H10 Case *)
   apply Z.geb_le in Case. (* Case *)
   lia.
-Abort.
+Qed.
 
 Lemma ERC20WrappedEth_transfer_oblg a0 a1 me d :
     ht_ft_cond a0 -> ht_valid_ft_cond a0 ->
@@ -186,6 +221,10 @@ code_proofs_auto.
 Qed.
 
 Lemma ERC20WrappedEth_transferFrom_vc a0 a1 a2 me d :
+    (forall a,
+      Int256Tree.get_default 0 a (ERC20WrappedEth_wrapped d)
+        < unattainableWeiAmount) ->
+    (toZ a2 < unattainableWeiAmount) ->
     ht_ft_cond a0 -> ht_valid_ft_cond a0 ->
     ht_ft_cond a1 -> ht_valid_ft_cond a1 ->
     ht_ft_cond a2 -> ht_valid_ft_cond a2 ->
@@ -193,11 +232,13 @@ Lemma ERC20WrappedEth_transferFrom_vc a0 a1 a2 me d :
     synth_func_cond ERC20WrappedEth_transferFrom ERC20WrappedEth_transferFrom_wf
                     a0 a1 a2 me d.
 Proof.
+intros Hextra1 Hextra2.
 intros.
 unfold synth_func_cond.
 simpl.
 repeat split.
-- remember ((@SpecTree.get
+- 
+remember ((@SpecTree.get
 (param_env
    (@cons hyper_type_pair int_U_pair
       (@cons hyper_type_pair int_U_pair
@@ -243,9 +284,30 @@ subst. simpl.
 unfold ht_ft_cond in H3.
 simpl in H3.
 inversion H14.
-clear -H3.
-simpl in *. unfold Z32 in a2. (* H3 *)
-shelve.
+simpl in *. unfold Z32 in a2.
+inversion H13.
+inversion H12.
+destruct(v >=? a2) eqn:SSSCase; [|simpl in H11; inversion H11].
+inversion H11.
+inversion H10.
+destruct(MachineModel.me_callvalue me =? 0) eqn:Case; [|simpl in H9; inversion H9].
+inversion H9.
+destruct(a2 >=? 0) eqn:SCase; [|simpl in H6; inversion H6].
+inversion H6.
+destruct(Int256.eq a0 a1) eqn:SSCase; [simpl in H8; inversion H8|].
+inversion H8.
+destruct(Int256.eq a0 (MachineModel.me_address me)) eqn:SSSSCase;
+  [simpl in H7; inversion H7|].
+inversion H7.
+subst.
+destruct m5. simpl in *.
+clear -Hextra2 Hextra1.
+unfold toZ, id in Hextra2.
+pose proof (Hextra1 a1) as H. (* Hextra1 Hextra2 H *)
+unfold Int256.modulus, two_power_nat. simpl.
+unfold Z_bounded in *.
+unfold unattainableWeiAmount, etherToWei in *.
+lia.
 - 
 remember ( (@SpecTree.get
 (param_env
@@ -291,7 +353,7 @@ rewrite <- H18 in Case.
 rewrite <- H19.
 clear -Case. (* Case *)
 lia.
-Abort.
+Qed.
 
 Lemma ERC20WrappedEth_transferFrom_oblg a0 a1 a2 me d :
     ht_ft_cond a0 -> ht_valid_ft_cond a0 ->
@@ -305,21 +367,67 @@ code_proofs_auto.
 Qed.
 
 Lemma ERC20WrappedEth_mint_vc me d :
+    (forall a,
+      Int256Tree.get_default 0 a (ERC20WrappedEth_wrapped d)
+        < unattainableWeiAmount) ->
+    (MachineModel.me_callvalue me < unattainableWeiAmount) ->
+    (ERC20WrappedEth__totalSupply d < unattainableWeiAmount) ->
     high_level_invariant d ->
     synth_func_cond ERC20WrappedEth_mint ERC20WrappedEth_mint_wf
                     me d.
 Proof.
+intros Hextra1 Hextra2 Hextra3.
 intros.
 unfold synth_func_cond.
 simpl.
 repeat split.
-- (* wrapped[msg_sender] := wrapped_amount + msg_value; *) 
+-
 inversion H2.
-shelve.
+destruct (Int256.eq
+(@MachineModel.me_caller
+   global_abstract_data_type
+   me)
+(@MachineModel.me_address
+   global_abstract_data_type
+   me)) eqn:Case; [simpl in H0; inversion H0|].
+inversion H0.
+destruct(Z.gtb
+(@MachineModel.me_callvalue
+   global_abstract_data_type
+   me) Z0); [|simpl in H1; inversion H1].
+inversion H1.
+subst.
+pose proof (Hextra1 (MachineModel.me_caller me)) as H3. (* Hextra1 Hextra2 H3 *)
+unfold Int256.modulus, two_power_nat. simpl.
+clear -Hextra1 Hextra2.
+pose proof (Hextra1 (MachineModel.me_caller me)).
+unfold Z_bounded in *. simpl in *.
+unfold unattainableWeiAmount, etherToWei in *.
+lia.
 - 
 inversion H4.
-shelve.
-Abort.
+inversion H3.
+inversion H2.
+destruct(Z.gtb
+(@MachineModel.me_callvalue
+   global_abstract_data_type
+   me) Z0); [|simpl in H1; inversion H1].
+inversion H1.
+destruct (Int256.eq
+(@MachineModel.me_caller
+   global_abstract_data_type
+   me)
+(@MachineModel.me_address
+   global_abstract_data_type
+   me)) eqn:Case; [simpl in H0; inversion H0|].
+inversion H0.
+subst.
+destruct m2. simpl in *.
+clear -Hextra2 Hextra3. (* Hextra2 Hextra3 *)
+unfold Int256.modulus, two_power_nat. simpl.
+unfold unattainableWeiAmount, etherToWei in *.
+lia.
+Qed.
 
 Lemma ERC20WrappedEth_mint_oblg me d :
     high_level_invariant d ->
@@ -330,11 +438,17 @@ code_proofs_auto.
 Qed.
 
 Lemma ERC20WrappedEth_burn_vc a0 me d :
+   (forall (a:Int256Tree.elt),
+      ERC20WrappedEth__totalSupply d
+      >=
+      Int256Tree.get_default 0 a (ERC20WrappedEth_wrapped d))
+   ->
     ht_ft_cond a0 -> ht_valid_ft_cond a0 ->
     high_level_invariant d ->
     synth_func_cond ERC20WrappedEth_burn ERC20WrappedEth_burn_wf
                     a0 me d.
 Proof.
+intros Hextra1.
 intros.
 unfold synth_func_cond.
 simpl in *.
@@ -357,16 +471,34 @@ lia.
 destruct(v >=? a0) eqn:Case; simpl in *; [|discriminate].
 rewrite Z.geb_le in Case.
 inversion H5. subst.
-clear -Case.
 remember ((@Int256Tree.get_default
 (@Z_bounded Int256.modulus modulus_bound) Z0
 (@MachineModel.me_caller global_abstract_data_type me)
 (ERC20WrappedEth_wrapped m3))) as wrapped_amount.
-assert(ERC20WrappedEth__totalSupply m6 >= wrapped_amount). (* .out -.g#* .g#1 -* Heqwrapped_amount *)
-shelve. (* Heqwrapped_amount Case H  *)
-clear -Case H.
+inversion H7.
+inversion H6.
+destruct(Z.eqb
+(@MachineModel.me_callvalue
+   global_abstract_data_type
+   me) Z0); [|simpl in H4; inversion H4].
+inversion H4.
+destruct (Int256.eq
+(@MachineModel.me_caller
+   global_abstract_data_type
+   me)
+(@MachineModel.me_address
+   global_abstract_data_type
+   me)) eqn:SCase; [simpl in H3; inversion H3|].
+inversion H3.
+destruct (a0 >=? 0); [|simpl in H2; inversion H2].
+inversion H2.
+subst.
+clear -Hextra1 Case.
+destruct m4. simpl in *.
+pose proof (Hextra1 (MachineModel.me_caller me)) as H.
+unfold Z_bounded in *. simpl in *. (* Hextra1 Case H *)
 lia.
-Abort.
+Qed.
 
 Lemma ERC20WrappedEth_burn_oblg a0 me d :
     ht_ft_cond a0 -> ht_valid_ft_cond a0 ->
